---
{"dg-publish":true,"permalink":"/Math/Probability Theory/Bayes' Theorem/","created":"2024-11-04T23:33:00.638-05:00","updated":"2024-11-10T21:50:15.739-05:00"}
---


#Math/Probability 

Bayes' Theorem states:
$$
P(A|B)=\frac{P(A)\cdot P(B|A)}{P(B)}
$$
## Proof

Recall from the formula for [[Math/Probability Theory/Multiplication Rule for Probability\|Multiplication Rule for Probability]]:
1. $P(A\cap B)=P(A)\cdot P(B|A)=P(B)\cdot P(A|B)$
2. To solve for $P(A|B)$ divide both sides by $P(B)$:
$$
P(A|B)=\frac{P(A)\cdot P(B|A)}{P(B)}
$$
