---
{"dg-publish":true,"permalink":"/Math/Algebra/Factoring (work in progress)/","created":"2024-10-04T02:07:40.453-04:00","updated":"2024-11-11T21:46:25.478-05:00"}
---

#Math/Algebra 

Factoring is the process of rewriting mathematical expressions as a product of several factors.

## Factoring Perfect Square Trinomials

Suppose you had a trinomial of the form:
$$
\begin{align}
a^2x^2+2abx+b^2=(ax+b)^2\\\\
\end{align}
$$
The above is what is known as a perfect square trinomial because it can be factored into the following form:
$$
\begin{align}
a^2x^2+2abx+b^2=(ax+b)^2\\\\
\end{align}
$$
### Example

Factor $4x^2+6x+9$

$$
\begin{align}
&\text{The above can be rewritten as $a^2x^2+abx+b^2=(2)^2x^2+2(2)(3)x+(3)^2$}\\\\
&=(2)^2x^2+(2)(3)x+(2)(3)x+(3)^2\\\\
&=2x(2x+3)+3(2x+3)\\\\
&=(2x+3)(2x+3)\\\\
&=(2x+3)^2
\end{align}
$$
## Factoring Other Trinomials


## Difference of Squares

Suppose you had an expression of the following form:

$$
a^2-b^2=(a+b)(a-b)
$$
To see why:
$$
\begin{align}
&(a+b)(a-b)\\\\
&=a^2-ab+ab-b^2&\text{Expand using the FOIL method}\\\\
&=a^2-b^2&\text{Simplify}
\end{align}
$$
### Example

Factor $16x^2-9$

$$
\begin{align}
16x^2 \text{ can be rewritten as $(4x)^2$ and $9$ can be rewritten as $3^2$}\\\\
16x^2-9=(4x)^2-(3)^2\\\\
=(4x+3)(4x-3)
\end{align}
$$